dsn/Lang/Dynamic/NStepStar.lean
@@ -1,34 +1,34 @@
 import Lang.Basic
 import Lang.Dynamic.EvalCon
-import Lang.Dynamic.Transition
+import Lang.Dynamic.NStep
 
 set_option pp.fieldNotation false
 
 
 namespace Lang.Dynamic
 
-inductive TransitionStar : Expr → Expr → Prop
-| refl e : TransitionStar e e
-| step e e' e'' : Transition e e' → TransitionStar e' e'' → TransitionStar e e''
+inductive NStepStar : Expr → Expr → Prop
+| refl e : NStepStar e e
+| step e e' e'' : NStep e e' → NStepStar e' e'' → NStepStar e e''
 
 
 
-theorem TransitionStar.econ_preservation
+theorem NStepStar.econ_preservation
   (econ : EvalCon E)
-  (transition_star : TransitionStar e e')
-: TransitionStar (E e) (E e')
+  (transition_star : NStepStar e e')
+: NStepStar (E e) (E e')
 := by induction transition_star with
 | refl e =>
   exact refl (E e)
 | step e e' e'' h0 h1 ih =>
-  apply TransitionStar.step
-  { exact Transition.econ econ h0 }
+  apply NStepStar.step
+  { exact NStep.econ econ h0 }
   { exact ih }
 
 
 
 def Confluent (a b : Expr) :=
-  ∃ e , TransitionStar a e ∧ TransitionStar b e
+  ∃ e , NStepStar a e ∧ NStepStar b e
 
 theorem Confluent.transitivity {a b c} :
   Confluent a b →
